iris/parameter.v
@@ -1,8 +1,11 @@
-Require Export modures.cmra.
+Require Export modures.cmra iris.language.
 
 Record iParam := IParam {
+  iexpr : Type;
+  ival : Type;
   istate : Type;
   icmra : cofeT → cmraT;
+  ilanguage : Language iexpr ival istate;
   icmra_empty A : Empty (icmra A);
   icmra_empty_spec A : RAIdentity (icmra A);
   icmra_map {A B} (f : A -n> B) : icmra A -n> icmra B;
@@ -12,6 +15,7 @@ Record iParam := IParam {
     icmra_map (g ◎ f) x ≡ icmra_map g (icmra_map f x);
   icmra_map_mono {A B} (f : A -n> B) : CMRAMonotone (icmra_map f)
 }.
+Existing Instances ilanguage.
 Existing Instances icmra_empty icmra_empty_spec icmra_map_ne icmra_map_mono.
 
 Lemma icmra_map_ext (Σ : iParam) {A B} (f g : A -n> B) m :
